Blanc.lean
@@ -1,7 +1,7 @@
 import Blanc.Solvent
 import Blanc.WethCode
 import Blanc.Ladder
-import Blanc.Flashmint
+import Blanc.Conserved
 import Blanc.FmintCode
 
 namespace Blanc
